Update F*

src/Comparse.Tactic.GenerateParser.fst
@@ -87,32 +87,6 @@ let parser_term_from_type_fv type_fv =
     pack (Tv_FVar (pack_fv parser_fullname))
   )
 
-// `tc (top_env ()) t` doesn't work with bound variables
-// and with splice there is no goal, so no `cur_env ()`
-val hacky_get_type: term -> Tac typ
-let hacky_get_type t =
-  match t with
-  | Tv_UInst fv _
-  | Tv_FVar fv -> tc (top_env ()) t
-  | Tv_Var bv -> type_of_bv bv
-  | _ -> fail "hacky_get_type: term is not a bv or a fv"
-
-val extract_bytes_impl: list term -> Tac (option bytes_impl)
-let extract_bytes_impl ts =
-  match ts with
-  | b::bl::_ -> (
-    let b_type = hacky_get_type b in
-    let bl_type = hacky_get_type bl in
-    let b_ok = (b_type `term_eq` (`Type0)) in
-    let bl_ok = (bl_type `term_eq` (mk_e_app (`bytes_like) [b])) in
-    if b_ok && bl_ok then (
-      Some (b, bl)
-    ) else (
-      None
-    )
-  )
-  | _ -> None
-
 val smart_mk_app_aux: term -> list term -> list binder -> Tac term
 let rec smart_mk_app_aux t args binders_to_copy =
   match args, binders_to_copy with
@@ -134,6 +108,20 @@ let smart_mk_app t args =
   let t_signature_binders, _ = collect_arr_bs t_signature in
   smart_mk_app_aux t args t_signature_binders
 
+val is_parametrized_by_bytes_typeclass: term -> Tac bool
+let is_parametrized_by_bytes_typeclass typ =
+  let typ_typ = tc (top_env ()) typ in
+  let (typ_typ_args, _) = collect_arr_bs typ_typ in
+  match typ_typ_args with
+  | b::bl::_ -> (
+    let b_type = type_of_binder b in
+    let bl_type = type_of_binder bl in
+    let b_ok = (b_type `term_eq` (`Type0)) in
+    let bl_ok = (bl_type `term_eq` (mk_e_app (`bytes_like) [binder_to_term b])) in
+    b_ok && bl_ok
+  )
+  | _ -> false
+
 val parser_from_type: bytes_impl -> term -> Tac parser_term
 let parser_from_type (bytes_term, bytes_like_term) t =
   let my_fail () = fail "parser_from_type: head given by `collect_app` is not a fv? (meta program don't handle parametric types, e.g. `option`)" in
@@ -144,9 +132,10 @@ let parser_from_type (bytes_term, bytes_like_term) t =
     let parser_unapplied = parser_term_from_type_fv fv in
     let parser_signature = tc (top_env ()) parser_unapplied in
     let expanded_type_args =
-      match extract_bytes_impl (List.Tot.map fst type_args) with
-      | Some _ -> type_args
-      | None -> (bytes_term, Q_Implicit)::(bytes_like_term, Q_Implicit)::type_args
+      if is_parametrized_by_bytes_typeclass type_unapplied then
+        type_args
+      else
+        (bytes_term, Q_Implicit)::(bytes_like_term, Q_Implicit)::type_args
     in
     (smart_mk_app parser_unapplied (List.Tot.map fst expanded_type_args), t)
   | Tv_Var _ -> (
@@ -206,12 +195,12 @@ let rec mk_destruct_pairs l =
   | [] -> (Pat_Constant C_Unit, [])
   | [h] -> (
     let bv_h = bv_of_binder h in
-    (Pat_Var bv_h, [bv_h])
+    (Pat_Var bv_h (seal (type_of_binder h)), [bv_h])
   )
   | h::t -> (
     let bv_h = bv_of_binder h in
     let (pattern_t, bv_t) = mk_destruct_pairs t in
-    let pattern = Pat_Cons (mkdtuple2_fv ()) None [(Pat_Var bv_h, false); (pattern_t, false)] in
+    let pattern = Pat_Cons (mkdtuple2_fv ()) None [(Pat_Var bv_h (seal (type_of_binder h)), false); (pattern_t, false)] in
     let bvs = bv_h::bv_t in
     (pattern, bvs)
   )
@@ -226,8 +215,8 @@ val mk_record_isomorphism_f: typ -> name -> list binder -> Tac term
 let mk_record_isomorphism_f result_type constructor_name constructor_binders =
   let (match_pattern, bvs) = mk_destruct_pairs constructor_binders in
   let match_body = mk_construct_record constructor_name bvs in
-  let x_bv = fresh_bv result_type in
-  pack (Tv_Abs (mk_binder x_bv) (pack (Tv_Match (pack (Tv_Var x_bv)) None [(match_pattern, match_body)])))
+  let x_bv = fresh_bv () in
+  pack (Tv_Abs (mk_binder x_bv result_type) (pack (Tv_Match (pack (Tv_Var x_bv)) None [(match_pattern, match_body)])))
 
 val mk_construct_pairs: list bv -> Tac term
 let rec mk_construct_pairs l =
@@ -239,11 +228,10 @@ let rec mk_construct_pairs l =
 
 val mk_record_isomorphism_g: typ -> name -> list binder -> Tac term
 let mk_record_isomorphism_g input_type constructor_name constructor_binders =
-  let bvs = Tactics.Util.map (fun b -> bv_of_binder b) constructor_binders in
-  let match_pattern = Pat_Cons (pack_fv constructor_name) None (List.Tot.map (fun bv -> (Pat_Var bv, false)) bvs) in
-  let match_body = mk_construct_pairs bvs in
-  let x_bv = fresh_bv input_type in
-  pack (Tv_Abs (mk_binder x_bv) (pack (Tv_Match (pack (Tv_Var x_bv)) None [(match_pattern, match_body)])))
+  let match_pattern = Pat_Cons (pack_fv constructor_name) None (Tactics.Util.map (fun b -> (Pat_Var (bv_of_binder b) (seal (type_of_binder b)), false)) constructor_binders) in
+  let match_body = mk_construct_pairs (Tactics.Util.map (fun b -> bv_of_binder b) constructor_binders) in
+  let x_bv = fresh_bv () in
+  pack (Tv_Abs (mk_binder x_bv input_type) (pack (Tv_Match (pack (Tv_Var x_bv)) None [(match_pattern, match_body)])))
 
 val dtuple2_ind: #a:Type -> #b:(a -> Type) -> p:((x:a & b x) -> Type0) -> squash (forall (x:a) (y:b x). p (|x, y|)) -> Lemma (forall xy. p xy)
 let dtuple2_ind #a #b p _ = ()
@@ -370,14 +358,14 @@ let get_tag_from_ctors ctors =
 val mk_tag_parser: bytes_impl -> typ -> list term -> Tac parser_term
 let mk_tag_parser bi tag_typ tag_vals =
   let pred =
-    let tag_bv = fresh_bv tag_typ in
+    let tag_bv = fresh_bv () in
     let tag_term = pack (Tv_Var tag_bv) in
     let mk_equality v1 v2 = mk_ie_app (`op_Equality) [tag_typ] [v1; v2] in
     let mk_disj value acc: Tac term = `(((`#(mk_equality tag_term value))) || (`#acc)) in
     guard (Cons? tag_vals);
     let tag_vals_head::tag_vals_tail = tag_vals in
     let disj = FStar.Tactics.fold_right mk_disj tag_vals_tail (`((`#(mk_equality tag_term tag_vals_head)))) in
-    pack (Tv_Abs (mk_binder tag_bv) disj)
+    pack (Tv_Abs (mk_binder tag_bv tag_typ) disj)
   in
   let (tag_parser, tag_typ) = parser_from_type bi tag_typ in
   (mk_ie_app (apply_implicit_bytes_impl (`refine) bi) [tag_typ] [tag_parser; pred], mk_e_app (`refined) [tag_typ; pred])
@@ -406,7 +394,7 @@ let mk_middle_sum_type_parser bi (tag_parser, tag_typ) tag_vals ctors =
       ctors
   in
   let (tag_to_pair_type_term, tag_to_pair_parser_term) =
-    let tag_bv = fresh_bv tag_typ in
+    let tag_bv = fresh_bv () in
     let tag_term = pack (Tv_Var tag_bv) in
     // Should be provable, but a dynamic check is enough
     guard (List.Tot.length tag_vals = List.Tot.length pair_parsers);
@@ -421,8 +409,8 @@ let mk_middle_sum_type_parser bi (tag_parser, tag_typ) tag_vals ctors =
       )
     in
     (
-      pack (Tv_Abs (mk_binder tag_bv) (pack (Tv_Match tag_term None branches_typ))),
-      pack (Tv_Abs (mk_binder tag_bv) (pack (Tv_Match tag_term None branches_term)))
+      pack (Tv_Abs (mk_binder tag_bv tag_typ) (pack (Tv_Match tag_term None branches_typ))),
+      pack (Tv_Abs (mk_binder tag_bv tag_typ) (pack (Tv_Match tag_term None branches_term)))
     )
   in
   let middle_parser = mk_ie_app (apply_implicit_bytes_impl (`bind) bi) [tag_typ; tag_to_pair_type_term] [tag_parser; tag_to_pair_parser_term] in
@@ -444,8 +432,9 @@ let mk_middle_to_sum_fun tag_typ tag_to_pair_typ tag_vals ctors =
       )
       (List.Pure.zip tag_vals ctors)
   in
-  let pair_bv = fresh_bv (mk_e_app (`dtuple2) [tag_typ; tag_to_pair_typ]) in
-  pack (Tv_Abs (mk_binder pair_bv) (pack (Tv_Match (pack (Tv_Var pair_bv)) None branches)))
+  let pair_bv = fresh_bv () in
+  let pair_typ = mk_e_app (`dtuple2) [tag_typ; tag_to_pair_typ] in
+  pack (Tv_Abs (mk_binder pair_bv pair_typ) (pack (Tv_Match (pack (Tv_Var pair_bv)) None branches)))
 
 val mk_sum_to_middle_fun: typ -> list term -> list ctor -> Tac term
 let mk_sum_to_middle_fun sum_typ tag_vals ctors =
@@ -454,16 +443,15 @@ let mk_sum_to_middle_fun sum_typ tag_vals ctors =
     Tactics.Util.map
       (fun (tag_val, (ctor_name, ctor_typ)) ->
         let (ctor_binders, _) = collect_arr_bs ctor_typ in
-        let bvs = Tactics.Util.map (fun b -> bv_of_binder b) ctor_binders in
-        let match_pattern = Pat_Cons (pack_fv ctor_name) None (List.Tot.map (fun bv -> (Pat_Var bv, false)) bvs) in
-        let pairs_term = mk_construct_pairs bvs in
+        let match_pattern = Pat_Cons (pack_fv ctor_name) None (Tactics.Util.map (fun b -> (Pat_Var (bv_of_binder b) (seal (binder_to_term b)), false)) ctor_binders) in
+        let pairs_term = mk_construct_pairs (Tactics.Util.map (fun b -> bv_of_binder b) ctor_binders) in
         let match_body = mk_e_app (`Mkdtuple2) [tag_val; pairs_term] in
         (match_pattern, match_body)
       )
       (List.Pure.zip tag_vals ctors)
   in
-  let sum_bv = fresh_bv sum_typ in
-  pack (Tv_Abs (mk_binder sum_bv) (pack (Tv_Match (pack (Tv_Var sum_bv)) None branches)))
+  let sum_bv = fresh_bv () in
+  pack (Tv_Abs (mk_binder sum_bv sum_typ) (pack (Tv_Match (pack (Tv_Var sum_bv)) None branches)))
 
 val refined_ind: a:Type -> pred:(a -> bool) -> p:(refined a pred -> Type0) -> squash (forall (x:a). pred x ==> p x) -> squash (forall (x:refined a pred). p x)
 let refined_ind a pred p _ = ()
@@ -608,13 +596,13 @@ let mk_tag_to_open_enum tag_typ ctors open_ctor =
       ctors
   in
   let branch_open =
-    let tag_bv = fresh_bv tag_typ in
+    let tag_bv = fresh_bv () in
     let (open_ctor_name, _) = open_ctor in
-    (Pat_Var tag_bv, mk_e_app (pack (Tv_FVar (pack_fv open_ctor_name))) [pack (Tv_Var tag_bv)])
+    (Pat_Var tag_bv (seal tag_typ), mk_e_app (pack (Tv_FVar (pack_fv open_ctor_name))) [pack (Tv_Var tag_bv)])
   in
   let branches = branches_closed @ [branch_open] in
-  let tag_bv = fresh_bv tag_typ in
-  pack (Tv_Abs (mk_binder tag_bv) (pack (Tv_Match (pack (Tv_Var tag_bv)) None branches)))
+  let tag_bv = fresh_bv () in
+  pack (Tv_Abs (mk_binder tag_bv tag_typ) (pack (Tv_Match (pack (Tv_Var tag_bv)) None branches)))
 
 val mk_open_enum_to_tag: typ -> typ -> list ctor -> ctor -> Tac term
 let mk_open_enum_to_tag tag_typ open_enum_typ ctors open_ctor =
@@ -630,13 +618,13 @@ let mk_open_enum_to_tag tag_typ open_enum_typ ctors open_ctor =
       ctors
   in
   let branch_open =
-    let tag_bv = fresh_bv tag_typ in
+    let tag_bv = fresh_bv () in
     let (open_ctor_name, _) = open_ctor in
-    (Pat_Cons (pack_fv open_ctor_name) None [Pat_Var tag_bv, false], pack (Tv_Var tag_bv))
+    (Pat_Cons (pack_fv open_ctor_name) None [Pat_Var tag_bv (seal tag_typ), false], pack (Tv_Var tag_bv))
   in
   let branches = branches_closed @ [branch_open] in
-  let x_bv = fresh_bv open_enum_typ in
-  pack (Tv_Abs (mk_binder x_bv) (pack (Tv_Match (pack (Tv_Var x_bv)) None branches)))
+  let x_bv = fresh_bv () in
+  pack (Tv_Abs (mk_binder x_bv open_enum_typ) (pack (Tv_Match (pack (Tv_Var x_bv)) None branches)))
 
 val mk_open_enum_isomorphism: bytes_impl -> parser_term -> typ -> list ctor -> ctor -> Tac parser_term
 let mk_open_enum_isomorphism bi (tag_parser, tag_typ) open_enum_typ ctors open_ctor =
@@ -682,8 +670,8 @@ let rec substitute_parser_in_term bi t =
       branches
     in
     pack (Tv_Match scrutinee ret new_branches)
-  | Tv_Let recf attrs bv def body ->
-    pack (Tv_Let recf attrs bv def (substitute_parser_in_term bi body))
+  | Tv_Let recf attrs bv ty def body ->
+    pack (Tv_Let recf attrs bv ty def (substitute_parser_in_term bi body))
   // Remove type ascription because sometimes F* gives us (...) <: Type0
   | Tv_AscribedC e c tac use_eq -> substitute_parser_in_term bi e
   | Tv_AscribedT e t tac use_eq -> substitute_parser_in_term bi e
@@ -704,14 +692,16 @@ val get_bytes_impl_and_parser_params: list binder -> Tac (bytes_impl & list bind
 let get_bytes_impl_and_parser_params params =
   let mk_bi_binders (): Tac (binder & binder) =
     let b = pack_binder {
-      binder_bv = (fresh_bv_named "bytes" (`Type0));
+      binder_bv = (fresh_bv_named "bytes");
       binder_qual = Q_Implicit;
       binder_attrs = [] ;
+      binder_sort = (`Type0);
     } in
     let bl = pack_binder {
-      binder_bv = (fresh_bv_named "bl" (`(bytes_like (`#(binder_to_term b)))));
+      binder_bv = (fresh_bv_named "bl");
       binder_qual = (Q_Meta (`FStar.Tactics.Typeclasses.tcresolve));
       binder_attrs = [];
+      binder_sort = (`(bytes_like (`#(binder_to_term b))));
     } in
     (b, bl)
   in
