src/Comparse.Tests.TacticFeatures.fst
@@ -206,7 +206,7 @@ type test_tag_unit =
 %splice [ps_test_tag_unit_is_well_formed] (gen_is_well_formed_lemma (`test_tag_unit))
 #pop-options
 
-#push-options "--fuel 0 --ifuel 1 --z3cliopt 'smt.qi.eager_threshold=0'"
+#push-options "--fuel 0 --ifuel 1 --z3cliopt 'smt.qi.eager_threshold=0' --z3rlimit 25"
 %splice [ps_test_tag_unit_length] (gen_length_lemma (`test_tag_unit))
 #pop-options
 
@@ -290,7 +290,7 @@ noeq type test_sum_num_annot (bytes:Type0) {|bytes_like bytes|} =
 %splice [ps_test_sum_num_annot] (gen_parser (`test_sum_num_annot))
 #pop-options
 
-#push-options "--fuel 0 --ifuel 1 --z3cliopt 'smt.qi.eager_threshold=0'"
+#push-options "--fuel 0 --ifuel 1 --z3cliopt 'smt.qi.eager_threshold=0' --z3rlimit 25"
 %splice [ps_test_sum_num_annot_is_well_formed] (gen_is_well_formed_lemma (`test_sum_num_annot))
 #pop-options
 
@@ -311,7 +311,7 @@ noeq type test_sum_with_num_annot (bytes:Type0) {|bytes_like bytes|} =
 %splice [ps_test_sum_with_num_annot] (gen_parser (`test_sum_with_num_annot))
 #pop-options
 
-#push-options "--fuel 0 --ifuel 1 --z3cliopt 'smt.qi.eager_threshold=0'"
+#push-options "--fuel 0 --ifuel 1 --z3cliopt 'smt.qi.eager_threshold=0' --z3rlimit 25"
 %splice [ps_test_sum_with_num_annot_is_well_formed] (gen_is_well_formed_lemma (`test_sum_with_num_annot))
 #pop-options
 
@@ -375,7 +375,7 @@ noeq type test_sum_dep (bytes:Type0) {|bytes_like bytes|} (n:nat) =
 %splice [ps_test_sum_dep] (gen_parser (`test_sum_dep))
 #pop-options
 
-#push-options "--fuel 0 --ifuel 1 --z3cliopt 'smt.qi.eager_threshold=0'"
+#push-options "--fuel 0 --ifuel 1 --z3cliopt 'smt.qi.eager_threshold=0' --z3rlimit 25"
 %splice [ps_test_sum_dep_is_well_formed] (gen_is_well_formed_lemma (`test_sum_dep))
 #pop-options
 
